SystemFD/Algorithm/TypeMatch.lean
@@ -1,0 +1,243 @@
+import SystemFD.Util
+import SystemFD.Term
+import SystemFD.Judgment
+import SystemFD.Ctx
+
+theorem option_lemma :
+  (∀ v, ¬ t = Option.some v) ->
+  t = .none
+:= by
+intro h
+cases t; simp
+case _ v => exfalso; apply h v rfl
+
+theorem neutral_form_rename {t : Term} (r : Ren) :
+  t.neutral_form = q ->
+  ([r.to]t).neutral_form = Option.map (λ (x, l) => (r x, List.map (λ (v, t) => (v, [r.to]t)) l)) q
+:= by
+intro h
+induction t generalizing r q
+any_goals try (simp at h; subst h; simp)
+case _ v t1 t2 ih1 ih2 =>
+  cases v; any_goals try solve | (simp at h; subst h; simp)
+  all_goals case _ =>
+    cases q
+    case _ =>
+      simp at h; simp; intro a b h2
+      have lem : t1.neutral_form = .none := by
+        apply option_lemma; intro v
+        apply h v.fst v.snd
+      replace ih1 := @ih1 .none r lem; simp at ih1
+      unfold Subst.apply at ih1; simp at ih1; rw [h2] at ih1
+      injection ih1
+    case _ v =>
+      simp at h; simp; rw [Option.bind_eq_some] at h
+      cases h; case _ a h =>
+      cases h; case _ h1 h2 =>
+        injection h2 with e; rw [Option.bind_eq_some]; subst e; simp
+        replace ih1 := ih1 r h1; simp at ih1
+        exists (r a.fst); exists (List.map (fun x => (x.fst, [r.to]x.snd)) a.snd)
+
+theorem stable_type_match_sound :
+  (τ, sR) = Term.to_telescope A ->
+  [S' τ.length]R = sR ->
+  .some (x, sp) = Term.neutral_form R ->
+  (Γ d@ x).is_stable ->
+  StableTypeMatch Γ A R
+:= by
+intro h1 h2 h3 h4
+induction A generalizing τ sR R x sp Γ <;> try simp at h1
+any_goals try (
+  case _ =>
+    cases h1; case _ e1 e2 =>
+      subst e1; subst e2
+      simp at h2; subst h2; constructor
+      apply h3; apply h4
+)
+case _ v t1 t2 ih1 ih2 =>
+  cases v <;> try simp at h1
+  any_goals try (
+    case _ =>
+      cases h1; case _ e1 e2 =>
+        subst e1; subst e2
+        simp at h2; subst h2; constructor
+        apply h3; apply h4
+  )
+  case all =>
+    cases τ
+    case _ => simp at h1
+    case _ hd τ =>
+      have lem1 : (τ, sR) = t2.to_telescope := by
+        cases h1; case _ u1 u2 =>
+          subst u2; injection u1 with _ e; subst e
+          generalize zdef : t2.to_telescope = z
+          apply Prod.eta
+      have lem2 : [S' τ.length][S]R = sR := by simp at h2; simp [*]
+      have lem3 :
+        .some (x + 1, List.map (λ (v, t) => (v, [S]t)) sp)
+        = ([S]R).neutral_form
+      := by
+        replace h3 := Eq.symm h3
+        have lem := neutral_form_rename (fun x => x + 1) h3
+        rw [Subst.to_S] at lem; rw [lem]; simp
+      have lem4 : ((Frame.kind t1 :: Γ)d@(x + 1)).is_stable := by
+        simp; rw [Frame.is_stable_stable]; apply h4
+      simp at h2; constructor
+      apply ih2 lem1 lem2 lem3 lem4
+  case arrow =>
+    cases τ
+    case _ => simp at h1
+    case _ hd τ =>
+      have lem1 : (τ, sR) = t2.to_telescope := by
+        cases h1; case _ u1 u2 =>
+          subst u2; injection u1 with _ e; subst e
+          generalize zdef : t2.to_telescope = z
+          apply Prod.eta
+      have lem2 : [S' τ.length][S]R = sR := by simp at h2; simp [*]
+      have lem3 :
+        .some (x + 1, List.map (λ (v, t) => (v, [S]t)) sp)
+        = ([S]R).neutral_form
+      := by
+        replace h3 := Eq.symm h3
+        have lem := neutral_form_rename (fun x => x + 1) h3
+        rw [Subst.to_S] at lem; rw [lem]; simp
+      have lem4 : ((Frame.type t1 :: Γ)d@(x + 1)).is_stable := by
+        simp; rw [Frame.is_stable_stable]; apply h4
+      simp at h2; constructor
+      apply ih2 lem1 lem2 lem3 lem4
+
+theorem telescope_empty {B : Term} :
+  ([], sB) = B.to_telescope ->
+  sB = B
+:= by
+intro h; induction B generalizing sB <;> simp at * <;> try simp [*]
+case _ v t1 t2 ih1 ih2 =>
+  cases v <;> simp at * <;> try simp [*]
+
+theorem telescope_valid_frames {B : Term} :
+  (f :: τ, sB) = B.to_telescope ->
+  (∃ t, f = .type t) ∨ (∃ t, f = .kind t)
+:= by
+intro h; induction B generalizing f τ sB <;> simp at *
+case _ v t1 t2 ih1 ih2 =>
+  cases v <;> simp at *
+  case _ => apply Or.inr; exists t1; apply h.1.1
+  case _ => apply Or.inl; exists t1; apply h.1.1
+
+theorem telescope_type_head {B : Term} :
+  (.type A :: τ, sB) = B.to_telescope ->
+  ∃ D, B = (A -t> D) ∧ (τ, sB) = D.to_telescope
+:= by
+intro h; induction B generalizing A τ sB <;> simp at *
+case _ v t1 t2 ih1 ih2 =>
+  cases v <;> simp at *
+  case _ =>
+    cases h; case _ h1 h2 =>
+    cases h1; case _ h1 h3 =>
+      subst h1; subst h2; subst h3
+      exists t2
+
+theorem telescope_kind_head {B : Term} :
+  (.kind A :: τ, sB) = B.to_telescope ->
+  ∃ D, B = (∀[A] D) ∧ (τ, sB) = D.to_telescope
+:= by
+intro h; induction B generalizing A τ sB <;> simp at *
+case _ v t1 t2 ih1 ih2 =>
+  cases v <;> simp at *
+  case _ =>
+    cases h; case _ h1 h2 =>
+    cases h1; case _ h1 h3 =>
+      subst h1; subst h2; subst h3
+      exists t2
+
+theorem telescope_rev_append_type :
+  Term.from_telescope_rev (Γ ++ [Frame.type A]) t = (A -t> (Term.from_telescope_rev Γ t))
+:= by sorry
+
+theorem telescope_rev_append_kind :
+  Term.from_telescope_rev (Γ ++ [Frame.kind A]) t = (∀[A] (Term.from_telescope_rev Γ t))
+:= by sorry
+
+theorem to_from_telescope {B : Term} :
+  (τ, sB) = B.to_telescope ->
+  sB.from_telescope τ = B
+:= by
+intro h; induction B generalizing τ sB <;> simp at *
+case bind2 v t1 t2 ih1 ih2 =>
+  cases v <;> simp at *
+  case all =>
+    cases h; case _ h1 h2 =>
+      subst h1; subst h2; simp
+      rw [telescope_rev_append_kind, ih2 rfl]
+  case arrow =>
+    cases h; case _ h1 h2 =>
+      subst h1; subst h2; simp
+      rw [telescope_rev_append_type, ih2 rfl]
+  all_goals (
+    cases h; case _ h1 h2 =>
+      subst h1; subst h2; simp)
+all_goals (
+  cases h; case _ h1 h2 =>
+    subst h1; subst h2; simp)
+
+theorem prefix_type_match_sound :
+  (τ, sR) = Term.to_telescope A ->
+  (τ', sT) = Term.to_telescope B ->
+  .some ξ = prefix_equal τ τ' ->
+  [S' τ.length]T = Term.from_telescope ξ sT ->
+  [S' τ.length]R = sR ->
+  .some (x, sp) = Term.neutral_form R ->
+  (Γ d@ x).is_stable ->
+  PrefixTypeMatch Γ A B T
+:= by
+intro h1 h2 h3 h4 h5 h6 h7
+induction τ, τ' using prefix_equal.induct generalizing Γ x sp sR R A sT B ξ T
+case _ t =>
+  simp at *; subst h3; subst h4
+  replace h1 := telescope_empty h1; subst h1; subst h5
+  have lem : sT.from_telescope ξ = B := by apply to_from_telescope h2
+  simp at lem; rw [lem]
+  apply PrefixTypeMatch.refl h6 h7
+case _ => simp at *
+case _ x1 t1 x2 t2 _ ih1 =>
+  simp at h3; cases h3; case _ h3e h3 =>
+    replace h3e := Frame.eq_of_beq h3e; subst h3e
+    have lem1 := telescope_valid_frames h2
+    cases lem1
+    case _ lem1 =>
+      cases lem1; case _ u lem1 =>
+        subst lem1
+        replace h1 := telescope_type_head h1
+        replace h2 := telescope_type_head h2
+        cases h1; case _ D1 h1 =>
+        cases h1; case _ h1 h1' =>
+        cases h2; case _ D2 h2 =>
+        cases h2; case _ h2 h2' =>
+          subst h1; subst h2; simp at h4; simp at h5
+          replace h6 := neutral_form_rename (fun x => x + 1) (Eq.symm h6); rw [Subst.to_S] at h6
+          simp at h6; constructor
+          replace ih1 := @ih1 sR D1 sT D2 ξ ([S]T) ([S]R) (x + 1)
+            (List.map (λ (v, t) => (v, [S]t)) sp) (.type u::Γ) h1' h2' h3
+          simp at ih1; replace ih1 := ih1 h4 h5 (Eq.symm h6)
+          apply ih1; rw [Frame.is_stable_stable]; apply h7
+    case _ lem1 =>
+      cases lem1; case _ u lem1 =>
+        subst lem1
+        replace h1 := telescope_kind_head h1
+        replace h2 := telescope_kind_head h2
+        cases h1; case _ D1 h1 =>
+        cases h1; case _ h1 h1' =>
+        cases h2; case _ D2 h2 =>
+        cases h2; case _ h2 h2' =>
+          subst h1; subst h2; simp at h4; simp at h5
+          replace h6 := neutral_form_rename (fun x => x + 1) (Eq.symm h6); rw [Subst.to_S] at h6
+          simp at h6; constructor
+          replace ih1 := @ih1 sR D1 sT D2 ξ ([S]T) ([S]R) (x + 1)
+            (List.map (λ (v, t) => (v, [S]t)) sp) (.kind u::Γ) h1' h2' h3
+          simp at ih1; replace ih1 := ih1 h4 h5 (Eq.symm h6)
+          apply ih1; rw [Frame.is_stable_stable]; apply h7
+case _ h =>
+  simp at h3; replace h := not_eq_of_beq h
+  cases h3; case _ h3e h3 =>
+    replace h3e := Frame.eq_of_beq h3e; subst h3e
+    exfalso; apply h rfl
