SystemFD/Metatheory/Substitution.lean
@@ -1,0 +1,97 @@
+import SystemFD.Term
+import SystemFD.Judgment
+import SystemFD.Ctx
+
+-- theorem lift_subst_rename (A : Term) :
+--   (∀ n y, σ n = .re y -> [σ](Γ d@ n) = Δ d@ y) ->
+--   (∀ n y, ^σ n = .re y -> [^σ]((A :: Γ) d@ n) = ([σ]A :: Δ) d@ y)
+-- := by
+-- intro h1 n y h2
+-- cases n
+-- case _ => simp at *; subst h2; simp
+-- case _ n =>
+--   simp at *; unfold Subst.compose at h2; simp at h2
+--   generalize ydef : σ n = y at *
+--   cases y <;> simp at h2
+--   case _ z =>
+--     subst h2; simp
+--     replace h1 := h1 n z ydef
+--     rw [<-Term.apply_compose, h1]
+
+-- theorem lift_subst_replace :
+--   Δ ⊢ ([σ]A) : .const K ->
+--   (∀ n t, σ n = .su t -> Δ ⊢ t : ([σ]Γ d@ n)) ->
+--   (∀ n t, ^σ n = .su t -> ([σ]A :: Δ) ⊢ t : ([^σ](A :: Γ) d@ n))
+-- := by
+-- intro j h1 n t h2
+-- cases n <;> simp at *
+-- case _ n =>
+--   unfold Subst.compose at h2; simp at h2
+--   generalize ydef : σ n = y at *
+--   cases y <;> simp at h2
+--   case _ t' =>
+--     replace h1 := h1 n t' ydef
+--     subst h2
+--     rw [<-Term.apply_compose]
+--     apply weaken; apply j; apply h1
+
+@[simp]
+abbrev idx_subst (σ : Subst Term) : JudgmentArgs v -> JudgmentArgs v :=
+  match v with
+  | .prf => λ (t, A) => ([σ]t, [σ]A)
+  | .wf => λ () => ()
+
+theorem subst :
+  (∀ n y, σ n = .re y -> (Γ d@ n).apply σ = Δ d@ y) ->
+  (∀ n t, σ n = .su t -> .some T = (Γ d@ n).get_type -> Δ ⊢ t : ([σ]T)) ->
+  Judgment v Γ idx ->
+  ⊢ Δ ->
+  Judgment v Δ (idx_subst σ idx)
+:= by
+intro h1 h2 j wf
+induction j generalizing Δ σ <;> simp at *
+case _ => sorry
+case _ => sorry
+case _ => sorry
+case _ => sorry
+case _ => sorry
+case _ => sorry
+case _ => sorry
+case _ => sorry
+case _ => sorry
+case _ => sorry
+case _ => sorry
+case _ => sorry
+case _ => sorry
+case _ => sorry
+case _ => sorry
+case _ => sorry
+case _ => sorry
+case _ => sorry
+case _ => sorry
+case _ => sorry
+case _ => sorry
+case _ => sorry
+case _ => sorry
+case _ => sorry
+case _ => sorry
+case _ => sorry
+case _ Γ p A τ sR R s t B τ' sT ξ sT' T K j1 j2 j3 j4 j5 j6 j7 j8 j9 j10 j11 ih1 ih2 ih3 ih4 ih5 =>
+  apply @Judgment.guard Δ ([σ]p) ([σ]A) (τ.apply σ) ([σ]sR) ([σ]R) ([σ]s) ([σ]t) ([σ]B)
+    (τ'.apply σ) ([σ]sT) ξ ([σ]sT') ([σ]T) K
+  apply ih1 h1 h2 wf
+  sorry
+case _ => sorry
+case _ => sorry
+case _ => sorry
+case _ => sorry
+case _ => sorry
+case _ => sorry
+case _ => sorry
+case _ => sorry
+case _ => sorry
+case _ => sorry
+case _ => sorry
+case _ => sorry
+case _ => sorry
+case _ => sorry
