SystemFD/Metatheory/TypeMatch.lean
@@ -1,0 +1,120 @@
+import SystemFD.Term
+import SystemFD.Judgment
+import SystemFD.Ctx
+
+theorem lift_subst_rename {Γ : Ctx Term} (A : Frame Term) :
+  (∀ n y, σ n = .re y -> (Γ d@ n).apply σ = Δ d@ y) ->
+  (∀ n y, ^σ n = .re y -> ((A :: Γ) d@ n).apply (^σ) = (A.apply σ :: Δ) d@ y)
+:= by
+intro h1 n y h2
+cases n
+case _ =>
+  simp at *; subst h2; simp
+  rw [Frame.apply_compose, Frame.apply_compose]; simp
+case _ n =>
+  simp at *; unfold Subst.compose at h2; simp at h2
+  generalize ydef : σ n = y at *
+  cases y <;> simp at h2
+  case _ z =>
+    subst h2; simp
+    replace h1 := h1 n z ydef
+    rw [Frame.apply_compose]; simp; rw [<-h1]
+    rw [Frame.apply_compose]
+
+theorem lift_subst_stable {σ : Subst Term} (A : Frame Term) :
+  (∀ n, (Γ d@ n).is_stable -> ∃ y, σ n = .re y) ->
+  (∀ n, ((A :: Γ) d@ n).is_stable → ∃ y, (^σ) n = .re y)
+:= by
+intro h1 n h2
+cases n <;> simp at *
+case _ n =>
+  rw [Frame.is_stable_stable] at h2
+  unfold Subst.compose; simp
+  replace h1 := h1 n h2
+  cases h1; case _ z h2 =>
+    rw [h2]; simp
+
+theorem neutral_form_subst {t : Term} (σ : Subst Term) :
+  (σ x = .re y) ->
+  t.neutral_form = .some (x, sp) ->
+  ([σ]t).neutral_form = .some (y, List.map (λ (v, l) => (v, [σ]l)) sp)
+:= by
+intro h1 h2
+induction t generalizing σ y x sp
+case ctor2 v t1 t2 ih1 ih2 =>
+  cases v; any_goals try simp at h2
+  all_goals
+    case _ =>
+    rw [Option.bind_eq_some] at h2
+    cases h2; case _ a h2 =>
+    cases h2; case _ h2 h3 =>
+      injection h3 with e; simp at *;
+      cases e; case _ e1 e2 =>
+        rw [Option.bind_eq_some]; subst e1; subst e2; simp
+        cases a; case _ ax asp =>
+          replace ih1 := ih1 σ h1 h2; simp at ih1
+          unfold Subst.apply at ih1; simp at ih1
+          exists y; exists (List.map (fun x => (x.fst, [σ]x.snd)) asp)
+all_goals simp at h2
+case _ z =>
+  cases h2; case _ e1 e2 =>
+    subst e1; subst e2; simp
+    rw [h1]; simp
+
+theorem stable_type_match_subst :
+  (∀ n y, σ n = .re y -> (Γ d@ n).apply σ = Δ d@ y) ->
+  (∀ n, (Γ d@ n).is_stable -> ∃ y, σ n = .re y) ->
+  StableTypeMatch Γ A B ->
+  StableTypeMatch Δ ([σ]A) ([σ]B)
+:= by
+intro h1 h2 j
+induction j generalizing Δ σ
+case _ sp Γ x R j1 j2 =>
+  replace h2 := h2 x j2
+  cases h2; case _ y h2 =>
+    replace j1 := neutral_form_subst σ h2 (Eq.symm j1); simp at j1
+    constructor; rw [j1]; rw [<-h1 x y h2, Frame.is_stable_stable]
+    apply j2
+case _ Γ A B R j ih =>
+  simp; constructor; simp
+  replace ih := @ih (^σ)
+    (((Frame.type A).apply σ) :: Δ)
+    (lift_subst_rename (Frame.type A) h1)
+    (lift_subst_stable (Frame.type A) h2)
+  simp at ih; apply ih
+case _ Γ A B R j ih =>
+  simp; constructor; simp
+  replace ih := @ih (^σ)
+    (((Frame.kind A).apply σ) :: Δ)
+    (lift_subst_rename (Frame.kind A) h1)
+    (lift_subst_stable (Frame.kind A) h2)
+  simp at ih; apply ih
+
+theorem prefix_type_match_subst :
+  (∀ n y, σ n = .re y -> (Γ d@ n).apply σ = Δ d@ y) ->
+  (∀ n, (Γ d@ n).is_stable -> ∃ y, σ n = .re y) ->
+  PrefixTypeMatch Γ A B T ->
+  PrefixTypeMatch Δ ([σ]A) ([σ]B) ([σ]T)
+:= by
+intro h1 h2 j
+induction j generalizing Δ σ
+case _ sp Γ x B T j1 j2 =>
+  replace h2 := h2 x j2
+  cases h2; case _ y h2 =>
+    replace j1 := neutral_form_subst σ h2 (Eq.symm j1); simp at j1
+    constructor; rw [j1]; rw [<-h1 x y h2, Frame.is_stable_stable]
+    apply j2
+case _ Γ A B V T j ih =>
+  simp; constructor; simp
+  replace ih := @ih (^σ)
+    (((Frame.type A).apply σ) :: Δ)
+    (lift_subst_rename (Frame.type A) h1)
+    (lift_subst_stable (Frame.type A) h2)
+  simp at ih; apply ih
+case _ Γ A B V T j ih =>
+  simp; constructor; simp
+  replace ih := @ih (^σ)
+    (((Frame.kind A).apply σ) :: Δ)
+    (lift_subst_rename (Frame.kind A) h1)
+    (lift_subst_stable (Frame.kind A) h2)
+  simp at ih; apply ih
