SystemFD/Metatheory/Weaken.lean
@@ -5,11 +5,16 @@ import SystemFD.Ctx
 theorem rename_lift r (A : Frame Term) :
   (∀ x, (Γ d@ x).apply r.to = Δ d@ (r x)) ->
   ∀ x, ((A::Γ) d@ x).apply r.lift.to = (A.apply r.to::Δ) d@ (Ren.lift r x)
-:= by sorry
--- intro h x; simp
--- cases x <;> simp at *
--- case _ => rw [Subst.lift_lemma]; simp
--- case _ x => rw [Subst.lift_lemma, <-h x]; simp
+:= by
+intro h x; simp
+cases x <;> simp at *
+case _ =>
+  rw [Subst.lift_lemma]; simp
+  rw [Frame.apply_compose, Frame.apply_compose]; simp
+case _ x =>
+  rw [Subst.lift_lemma, <-h x]; simp
+  rw [Frame.apply_compose, Frame.apply_compose]; simp
+
 
 @[simp]
 abbrev idx_ren (r : Ren) : JudgmentArgs v -> JudgmentArgs v :=
@@ -47,6 +52,12 @@ case _ => sorry
 case _ => sorry
 case _ => sorry
 case _ => sorry
+case _ Γ p A τ sR R s t B τ' sT ξ sT' T K j1 j2 j3 j4 j5 j6 j7 j8 j9 j10 j11 ih1 ih2 ih3 ih4 ih5 =>
+  sorry
+  -- apply @Judgment.guard Δ ([r.to]p) ([r.to]A) τ ([r.to]sR) ([r.to]R) ([r.to]s) ([r.to]t)
+  --   ([r.to]B) τ' ([r.to]sT) ξ ([r.to]sT') ([r.to]T) K
+  -- apply ih1 r wf h
+  -- sorry
 case _ => sorry
 case _ => sorry
 case _ => sorry
@@ -61,4 +72,95 @@ case _ => sorry
 case _ => sorry
 case _ => sorry
 case _ => sorry
-case _ => sorry
+
+theorem weaken_empty :
+  Γ ⊢ t : A ->
+  (.empty::Γ) ⊢ ([S]t) : ([S]A)
+:= by
+intro j; apply rename _ j
+case _ => constructor; apply judgment_ctx_wf j
+case _ => intro x; simp; rw [Subst.to_S]
+
+theorem weaken_type :
+  Γ ⊢ T : .const K ->
+  Γ ⊢ t : A ->
+  (.type T::Γ) ⊢ ([S]t) : ([S]A)
+:= by
+intro j1 j2; apply rename _ j2
+case _ => constructor; apply j1; apply judgment_ctx_wf j1
+case _ => intro x; simp; rw [Subst.to_S]
+
+theorem weaken_kind :
+  Γ ⊢ T : .kind ->
+  Γ ⊢ t : A ->
+  (.kind T::Γ) ⊢ ([S]t) : ([S]A)
+:= by
+intro j1 j2; apply rename _ j2
+case _ => constructor; apply j1; apply judgment_ctx_wf j1
+case _ => intro x; simp; rw [Subst.to_S]
+
+theorem weaken_datatype :
+  Γ ⊢ T : .kind ->
+  Γ ⊢ t : A ->
+  (.datatype T::Γ) ⊢ ([S]t) : ([S]A)
+:= by
+intro j1 j2; apply rename _ j2
+case _ => constructor; apply j1; apply judgment_ctx_wf j1
+case _ => intro x; simp; rw [Subst.to_S]
+
+theorem weaken_ctor :
+  Γ ⊢ T : ★ ->
+  valid_ctor Γ ->
+  Γ ⊢ t : A ->
+  (.ctor T::Γ) ⊢ ([S]t) : ([S]A)
+:= by
+intro j1 j2 j3; apply rename _ j3
+case _ => constructor; apply j1; apply judgment_ctx_wf j1; apply j2
+case _ => intro x; simp; rw [Subst.to_S]
+
+theorem weaken_opent :
+  Γ ⊢ T : .kind ->
+  Γ ⊢ t : A ->
+  (.opent T::Γ) ⊢ ([S]t) : ([S]A)
+:= by
+intro j1 j2; apply rename _ j2
+case _ => constructor; apply j1; apply judgment_ctx_wf j1
+case _ => intro x; simp; rw [Subst.to_S]
+
+theorem weaken_openm :
+  Γ ⊢ T : .const K ->
+  Γ ⊢ t : A ->
+  (.openm T::Γ) ⊢ ([S]t) : ([S]A)
+:= by
+intro j1 j2; apply rename _ j2
+case _ => constructor; apply j1; apply judgment_ctx_wf j1
+case _ => intro x; simp; rw [Subst.to_S]
+
+theorem weaken_insttype :
+  Γ ⊢ T : .const K ->
+  Γ ⊢ t : A ->
+  (.openm T::Γ) ⊢ ([S]t) : ([S]A)
+:= by
+intro j1 j2; apply rename _ j2
+case _ => constructor; apply j1; apply judgment_ctx_wf j1
+case _ => intro x; simp; rw [Subst.to_S]
+
+theorem weaken_inst :
+  .openm T = Γ d@ x ->
+  Γ ⊢ b : T ->
+  Γ ⊢ t : A ->
+  (.inst x b::Γ) ⊢ ([S]t) : ([S]A)
+:= by
+intro j1 j2 j3; apply rename _ j3
+case _ => constructor; apply j1; apply j2; apply judgment_ctx_wf j2
+case _ => intro x; simp; rw [Subst.to_S]
+
+theorem weaken_term :
+  Γ ⊢ T : .const K ->
+  Γ ⊢ b : T ->
+  Γ ⊢ t : A ->
+  (.term T b::Γ) ⊢ ([S]t) : ([S]A)
+:= by
+intro j1 j2 j3; apply rename _ j3
+case _ => constructor; apply j1; apply j2; apply judgment_ctx_wf j2
+case _ => intro x; simp; rw [Subst.to_S]
