SystemFD/Term/VariableSet.lean
@@ -1,0 +1,25 @@
+import SystemFD.Substitution
+import SystemFD.Ctx
+import SystemFD.Term.Definition
+
+namespace List
+  @[simp]
+  def inter [BEq T] (l1 l2 : List T) : List T := filter (elem · l2) l1
+end List
+
+namespace Term
+  @[simp]
+  def vars : Term -> List Nat
+  | var x => [x]
+  | kind => []
+  | const _ => []
+  | ctor1 _ t => vars t
+  | ctor2 _ t1 t2 => vars t1 ++ vars t2
+  | bind2 _ t1 t2 => vars t1 ++ vars t2
+  | ite t1 t2 t3 t4 => vars t1 ++ vars t2 ++ vars t3 ++ vars t4
+  | guard t1 t2 t3 => vars t1 ++ vars t2 ++ vars t3
+  | letdata t1 t2 => vars t1 ++ vars t2
+  | letterm t1 t2 t3 => vars t1 ++ vars t2 ++ vars t3
+  | inst _ t1 t2 => vars t1 ++ vars t2
+  | decl t => vars t
+end Term
