SystemFD/Util.lean
@@ -5,14 +5,15 @@ def prefix_equal [BEq T] : List T -> List T -> Option (List T)
 | .cons _ _, [] => .none
 | .cons x1 t1, .cons x2 t2 => if x1 == x2 then prefix_equal t1 t2 else .none
 
-
-instance : Monad List where -- This seems fishy. Why doesn't lean have a Monad List instance?
+instance : Monad List where
   pure a := List.cons a List.nil
   bind l f := List.flatMap l f
-
 
 theorem option_neg : (∀ l, ¬ (p = some l)) -> p = none := by
   intros np;
   cases p;
   case _ => simp
   case _ v => simp; exfalso; apply np v; rfl
+
+theorem not_eq_of_beq [BEq T] [LawfulBEq T] {x y : T} : ¬ ((x == y) = true) -> x ≠ y := by
+intro h1 h2; subst h2; apply h1; apply LawfulBEq.rfl
